secure_api/hkdf/Crypto.HMAC.fst
@@ -11,14 +11,14 @@ noextract
 let wrap (a:alg) (key: bseq{Seq.length key <= maxLength a}): 
   Tot (lbseq (blockLength a))
 = 
-  let key0 = if length key <= blockLength a then key else hash a key in 
+  let key0 = if length key <= blockLength a then key else spec a key in 
   let paddingLength = blockLength a - length key0 in 
   key0 @| Seq.create paddingLength 0uy
 
 private let wrap_lemma (a: alg) (key: bseq{Seq.length key <= maxLength a}): Lemma
   (requires length key > blockLength a)
   (ensures wrap a key == (
-    let key0 = hash a key in
+    let key0 = spec a key in
     let paddingLength = blockLength a - length key0 in 
     key0 @| Seq.create paddingLength 0uy)) = ()
 
@@ -40,8 +40,8 @@ let hmac a key data =
 /// HACL*.
 
 open FStar.HyperStack.All
-open FStar.Buffer
 open FStar.UInt32
+open FStar.Buffer
 
 module ST = FStar.HyperStack.ST
 
@@ -65,11 +65,11 @@ val wrap_key:
 [@"substitute"]
 let wrap_key a output key len =
   let i = if len <=^ blockLen a then len else tagLen a in 
-  let nkey = Buffer.sub output 0ul i in 
-  let pad = Buffer.sub output i (blockLen a -^ i) in
+  let nkey = sub output 0ul i in 
+  let pad = sub output i (blockLen a -^ i) in
   let h0 = ST.get () in
   if len <=^ blockLen a then 
-    Buffer.blit key 0ul nkey 0ul len
+    blit key 0ul nkey 0ul len
   else 
     Hash.compute a len key nkey;
   let h1 = ST.get () in
@@ -83,7 +83,7 @@ let wrap_key a output key len =
 val part1:
   a: alg ->
   acc: state a -> ( 
-  let uint = if a = SHA256 then UInt32.t else UInt64.t in 
+  let uint = state_word a in 
   s2: lbptr (blockLength a) ->
   data: bptr {
     length data + blockLength a  < pow2 32 /\ 
@@ -101,67 +101,74 @@ val part1:
       modifies_2 #uint acc s2 h0 h1 /\ (
       let hash0 = Seq.slice (as_seq h1 s2) 0 (tagLength a) in
       hash0 == spec a (Seq.append (as_seq h0 s2) (as_seq h0 data))))))
-
+ 
 #reset-options "--max_fuel 0 --z3rlimit 1000"
 [@"substitute"]
-let part1 a (acc: state a) keyblock data len =
-  Math.Lemmas.lemma_div_mod (v len) (blockLength a);
-  let n0 = len /^ blockLen a in
-  let r0 = len %^ blockLen a in
-  let data_blocks = Buffer.sub data 0ul (n0 *^ blockLen a) in
-  let data_last = Buffer.offset data (n0 *^ blockLen a) in
+let part1 a (acc: state a) key data len =
+  let ll = len %^ blockLen a in
+  let lb = len -^ ll in
+  let blocks = Buffer.sub data 0ul lb in
+  let last = Buffer.offset data lb in
   Hash.init a acc;  
-  Hash.update a acc keyblock;
+  Hash.update a acc key;
   let h1 = ST.get() in 
-  Hash.update_multi a acc data_blocks (n0 *^ blockLen a);
+  Hash.update_multi a acc blocks lb;
   let h2 = ST.get() in
-  Hash.update_last a acc data_last (blockLen a +^ len);
+  Hash.update_last a acc last (blockLen a +^ len);
   let h3 = ST.get() in
-  let tag = Buffer.sub keyblock 0ul (tagLen a) in (* Salvage memory *)
+  let tag = Buffer.sub key 0ul (tagLen a) in (* Salvage memory *)
   Hash.extract a acc tag; 
   (
-    let v1 = as_seq h1 keyblock in 
-    let vblocks = as_seq h1 data_blocks in 
+    let p = blockLength a in 
+    let key1 = as_seq h1 key in 
+    let blocks1 = as_seq h1 blocks in 
     let acc1 = as_acc h1 acc in 
-    lemma_compress (acc0 #a) v1;
-    assert(acc1 == hash0 #a v1);
-    let v2 = v1 @| vblocks in 
+    lemma_compress (acc0 #a) key1;
+    assert(acc1 == hash0 #a key1);
+    let v2 = key1 @| blocks1 in 
     let acc2 = as_acc h2 acc in 
-    lemma_hash2 (acc0 #a) v1 vblocks;
+    // assert (Seq.length key1 % p = 0);
+    // assert (Seq.length blocks1 % p = 0);
+    // assert (Seq.length v2 % p = 0);
+    lemma_hash2 (acc0 #a) key1 blocks1;
     assert(acc2 == hash0 #a v2);
-    let vdata = as_seq h1 data in  
-    let vlast = as_seq h1 data_last in 
-    let vsuffix = suffix a (blockLength a + v len) in 
-    Seq.lemma_eq_intro vdata (vblocks @| vlast);
+    let data1 = as_seq h1 data in  
+    let last1 = as_seq h1 last in 
+    let suffix1 = suffix a (p + v len) in 
+    Seq.lemma_eq_intro data1 (blocks1 @| last1);
     let acc3 = as_acc h3 acc in 
-    lemma_hash2 (acc0 #a) v2 (vlast @| vsuffix); 
-    assert(acc3 == hash0 #a (v2 @| (vlast @| vsuffix)));
-    Seq.append_assoc v2 vlast vsuffix; 
-    Seq.append_assoc v1 vblocks vlast;
-    assert(acc3 == hash0 #a ((v1 @| vdata) @| vsuffix));
-    assert(finish acc3 == spec a (v1 @| vdata)))
-  
+    let ls = Seq.length suffix1 in 
+    assert((p + v len + ls) % p = 0);
+    Math.Lemmas.lemma_mod_plus (v ll + ls) (1 + v len / p) p;
+    assert((v ll + ls) % p = 0);
+    lemma_hash2 (acc0 #a) v2 (last1 @| suffix1); 
+    assert(acc3 == hash0 #a (v2 @| (last1 @| suffix1)));
+    Seq.append_assoc v2 last1 suffix1; 
+    Seq.append_assoc key1 blocks1 last1;
+    assert(acc3 == hash0 #a ((key1 @| data1) @| suffix1));
+    assert(finish acc3 == spec a (key1 @| data1))
+    )
+
 // the two parts have the same stucture; let's keep their proofs in sync. 
 [@"substitute"]
 val part2:
   a: alg ->
-  acc: state a -> ( 
-  let uint = if a = SHA256 then UInt32.t else UInt64.t in 
+  acc: state a ->  
   mac: lbptr (tagLength a) ->
   opad: lbptr (blockLength a) ->
   tag: lbptr (tagLength a) {disjoint mac opad /\ disjoint mac tag} ->
   Stack unit
     (requires fun h0 -> 
-      disjoint #uint acc opad /\ 
-      disjoint #uint acc tag /\ 
-      disjoint #uint acc mac /\ 
-      live #uint h0 acc /\ 
+      disjoint acc opad /\ 
+      disjoint acc tag /\ 
+      disjoint acc mac /\ 
+      live h0 acc /\ 
       live h0 mac /\ live h0 opad /\ live h0 tag)
     (ensures fun h0 _ h1 -> 
-      live h1 mac /\ live h0 mac /\ modifies_2 #uint acc mac h0 h1 /\
+      live h1 mac /\ live h0 mac /\ modifies_2 acc mac h0 h1 /\
       ( let payload = Seq.append (as_seq h0 opad) (as_seq h0 tag) in 
         Seq.length payload <= maxLength a /\
-        as_seq h1 mac = spec a payload)))
+        as_seq h1 mac = spec a payload))
 
 [@"substitute"]
 let part2 a acc mac opad tag =
@@ -178,20 +185,18 @@ let part2 a acc mac opad tag =
     let acc1 = as_acc h1 acc in 
     lemma_compress (acc0 #a) v1;
     assert(acc1 == hash0 #a v1);
-    let vtag = as_seq h1 tag in 
-    let vsuffix = suffix a (blockLength a + tagLength a) in
+    let tag1 = as_seq h1 tag in 
+    let suffix1 = suffix a (blockLength a + tagLength a) in
     let acc2 = as_acc h2 acc in 
-    lemma_hash2 (acc0 #a) v1 (vtag @| vsuffix); 
-    Seq.append_assoc v1 vtag vsuffix;
-    assert(acc2 == hash0 #a ((v1 @| vtag) @| vsuffix));
-    assert(finish acc2 = spec a (v1 @| vtag)))
+    lemma_hash2 (acc0 #a) v1 (tag1 @| suffix1); 
+    Seq.append_assoc v1 tag1 suffix1;
+    assert(acc2 == hash0 #a ((v1 @| tag1) @| suffix1));
+    assert(finish acc2 = spec a (v1 @| tag1)))
 
 // similar spec as hmac with keylen = blockLen a 
-[@"substitute"]
 val hmac_core:
   a: alg ->
   acc: state a -> (
-  let uint = if a = SHA256 then UInt32.t else UInt64.t in 
   tag: lbptr (tagLength a) ->
   key: lbptr (blockLength a) {disjoint key tag} ->
   data: bptr{
@@ -201,23 +206,22 @@ val hmac_core:
   datalen: UInt32.t {v datalen = length data} ->
   Stack unit
   (requires fun h0 -> 
-    disjoint #uint acc tag /\ 
-    disjoint #uint acc key /\ 
-    disjoint #uint acc data /\ 
-    live #uint h0 acc /\ 
+    disjoint acc tag /\ 
+    disjoint acc key /\ 
+    disjoint acc data /\ 
+    live h0 acc /\ 
     live h0 tag /\ live h0 key /\ live h0 data)
   (ensures fun h0 _ h1 ->   
     live h1 tag /\ live h0 tag /\
     live h1 key /\ live h0 key /\
     live h1 data /\ live h0 data /\ 
-    //modifies_2 #uint acc tag h0 h1 /\
+    modifies_2 acc tag h0 h1 /\
     ( let k = as_seq h0 key in  
       let k1 = xor k 0x36uy in
       let k2 = xor k 0x5cuy in
       let v1 = spec a (k1 @| as_seq h0 data) in 
       Seq.length (k2 @| v1) <= maxLength a /\
       as_seq h1 tag = spec a (k2 @| v1))))
-      //harder: hmac a (as_seq h0 key) (as_seq h0 data)
 
 // todo functional correctness.
 // below, we only XOR with a constant bytemask.
@@ -236,6 +240,7 @@ let xor_bytes_inplace a b len =
 // mac, so that we can reuse the pad.
 [@"substitute"]
 let hmac_core a acc mac key data len =
+  let h00 = ST.get() in 
   push_frame ();
   let ipad = Buffer.create 0x36uy (blockLen a) in
   let opad = Buffer.create 0x5cuy (blockLen a) in
@@ -260,32 +265,41 @@ let hmac_core a acc mac key data len =
     assume(as_seq h0 ipad = k1); 
     assume(as_seq h1 opad = k2);
     assert(v1 == spec a (k1 @| vdata));
-    assert(v2 == spec a (k2 @| v1)));
-  pop_frame ()
-  
+    assert(v2 == spec a (k2 @| v1));
+
+    assert(modifies_2 acc ipad h0 h1); 
+    assert(modifies_2 acc mac h1 h2));
+  pop_frame ();
+  let h3 = ST.get() in 
+  assume(modifies_2 acc mac h00 h3) //18-04-14 still no convenient way to prove those? 
+
 
 // not much point in separating hmac_core? verbose, but it helps
 // monomorphise stack allocations.
 
 let compute a mac key keylen data datalen =
   push_frame (); 
-  let keyblock = Buffer.create 0x00uy (blockLen a) in
   assert_norm(pow2 32 <= maxLength a);
-  wrap_key a keyblock key keylen;
   ( match a with 
   | SHA256 -> 
       push_frame();
-      let acc = Buffer.create 0ul (state_size a) in 
+      let keyblock = Buffer.create 0x00uy (blockLen a) in
+      wrap_key a keyblock key keylen;
+      let acc = Buffer.create (state_zero a) (state_size a) in 
       hmac_core SHA256 acc mac keyblock data datalen;
       pop_frame()
   | SHA384 -> 
       push_frame();
-      let acc = Buffer.create 0UL (state_size a) in 
+      let keyblock = Buffer.create 0x00uy (blockLen a) in
+      wrap_key a keyblock key keylen;
+      let acc = Buffer.create (state_zero a) (state_size a) in 
       hmac_core SHA384 acc mac keyblock data datalen;
       pop_frame()
   | SHA512 -> 
       push_frame();
-      let acc = Buffer.create 0UL (state_size a) in 
+      let keyblock = Buffer.create 0x00uy (blockLen a) in
+      wrap_key a keyblock key keylen;
+      let acc = Buffer.create (state_zero a) (state_size a) in 
       hmac_core SHA512 acc mac keyblock data datalen;
       pop_frame());
   pop_frame ()
